Verify some helper functions using map.for_range; need better support

src/proof/iam_model/example/util.v
@@ -1,4 +1,5 @@
 From New.proof Require Import prelude empty_ffi.
+From New.proof.map Require Import for_range.
 From New.proof.iam_model Require Export example_init.
 From New.code.iam_model Require Export example.
 From iris.algebra Require Import gmap gset.
@@ -13,6 +14,240 @@ Definition policy_ids_for_identity
     (abs_identities : gmap iammodel.IdentityID.t (gmap iammodel.PolicyID.t unit))
     (identity : iammodel.IdentityID.t) : gmap iammodel.PolicyID.t unit :=
   default (∅ : gmap iammodel.PolicyID.t unit) (abs_identities !! identity).
+
+Definition identity_has_policy_for_resource
+    (abs_identities : gmap iammodel.IdentityID.t (gmap iammodel.PolicyID.t unit))
+    (policies : gmap iammodel.PolicyID.t iammodel.IdentityPolicy.t)
+    (resource : iammodel.ResourceName.t)
+    (identity : iammodel.IdentityID.t) : bool :=
+  match abs_identities !! identity with
+  | Some policy_ids =>
+      bool_decide (attached_policies_for_resource policies policy_ids resource ≠ ∅)
+  | None => false
+  end.
+
+Lemma attached_policies_for_resource_elem
+    policies policy_ids resource policy_id :
+  policy_id ∈ attached_policies_for_resource policies policy_ids resource ↔
+  policy_ids !! policy_id = Some tt ∧
+  policy_matches_resource policies resource policy_id = true.
+Proof.
+  unfold attached_policies_for_resource.
+  rewrite elem_of_dom.
+  split.
+  - intros [[] Hlookup].
+    apply map_lookup_filter_Some in Hlookup as [Hlookup Hmatches].
+    split; done.
+  - intros [Hlookup Hmatches].
+    exists tt. apply map_lookup_filter_Some. split; done.
+Qed.
+
+Lemma attached_policies_for_resource_empty
+    policies policy_ids resource :
+  (∀ policy_id,
+    policy_ids !! policy_id = Some tt →
+    policy_matches_resource policies resource policy_id = false) →
+  attached_policies_for_resource policies policy_ids resource = ∅.
+Proof.
+  intros Hnone. apply set_eq. intros policy_id.
+  rewrite elem_of_empty attached_policies_for_resource_elem.
+  split; [|done].
+  intros [Hlookup Hmatches].
+  rewrite (Hnone policy_id Hlookup) in Hmatches. done.
+Qed.
+
+Lemma current_key_not_in_take `{EqDecision A} `{Countable A} (keys : list A) i key :
+  NoDup keys →
+  keys !! Z.to_nat i = Some key →
+  (0 ≤ i)%Z →
+  key ∉ list_to_set (C:=gset A) (take (Z.to_nat i) keys).
+Proof.
+  intros Hnodup Hlookup Hi_nonneg Hin.
+  rewrite elem_of_list_to_set in Hin.
+  apply list_elem_of_lookup_1 in Hin as [j Htake_lookup].
+  apply lookup_take_Some in Htake_lookup as [Hlookup_j Hj].
+  pose proof (NoDup_lookup _ _ _ _ Hnodup Hlookup_j Hlookup) as ->.
+  lia.
+Qed.
+
+Lemma filtered_key_list_dom
+    (keys : list iammodel.IdentityID.t)
+    (phys_identities : gmap iammodel.IdentityID.t map.t)
+    (abs_identities : gmap iammodel.IdentityID.t (gmap iammodel.PolicyID.t unit))
+    policies resource :
+  list_to_set keys = dom phys_identities →
+  dom phys_identities = dom abs_identities →
+  list_to_set (C:=gset iammodel.IdentityID.t)
+    (filter (λ identity,
+      identity_has_policy_for_resource abs_identities policies resource identity)
+      keys) =
+  dom (filter (λ '(_, policy_ids),
+    attached_policies_for_resource policies policy_ids resource ≠ ∅)
+    abs_identities).
+Proof.
+  intros Hkeys_dom Hdom_eq.
+  apply set_eq. intros identity.
+  rewrite elem_of_list_to_set elem_of_dom.
+  split.
+  - intros Hin.
+    apply list_elem_of_filter in Hin as [Hmatches Hidentity_keys].
+    unfold identity_has_policy_for_resource in Hmatches.
+    destruct (abs_identities !! identity) as [policy_ids|] eqn:Hlookup;
+      [|done].
+    destruct (bool_decide
+      (attached_policies_for_resource policies policy_ids resource ≠ ∅))
+      eqn:Hmatches_eq; [|done].
+    apply bool_decide_eq_true in Hmatches_eq.
+    exists policy_ids. apply map_lookup_filter_Some. split; done.
+  - intros [policy_ids Hlookup].
+    apply map_lookup_filter_Some in Hlookup as [Hlookup Hnonempty].
+    apply list_elem_of_filter. split.
+    + unfold identity_has_policy_for_resource. rewrite Hlookup.
+      destruct (bool_decide_reflect
+        (attached_policies_for_resource policies policy_ids resource ≠ ∅));
+        done.
+    + assert (identity ∈ list_to_set (C:=gset iammodel.IdentityID.t) keys)
+        as Hin_keys.
+      { rewrite Hkeys_dom Hdom_eq elem_of_dom.
+        eexists. exact Hlookup. }
+      rewrite elem_of_list_to_set in Hin_keys. exact Hin_keys.
+Qed.
+
+Lemma wp_hasPolicyForResource
+    policy_ids_l policies_l
+    (policy_ids : gmap iammodel.PolicyID.t unit)
+    (policies : gmap iammodel.PolicyID.t iammodel.IdentityPolicy.t)
+    resource dq_policy_ids dq_policies :
+  {{{ "#Hpkg" ∷ is_pkg_init example ∗
+      "HpolicyIDs" ∷ policy_ids_l ↦${dq_policy_ids} policy_ids ∗
+      "Hpolicies" ∷ policies_l ↦${dq_policies} policies
+  }}}
+    @! example.hasPolicyForResource #policy_ids_l #policies_l #resource
+  {{{ RET #(bool_decide
+        (attached_policies_for_resource policies policy_ids resource ≠ ∅));
+      "HpolicyIDs" ∷ policy_ids_l ↦${dq_policy_ids} policy_ids ∗
+      "Hpolicies" ∷ policies_l ↦${dq_policies} policies
+  }}}.
+Proof.
+  wp_start as "H".
+  iNamed "H".
+  wp_auto.
+  wp_apply (wp_map_for_range_return_or_return (key_type:=iammodel.PolicyID)
+    (λ (keys : list iammodel.PolicyID.t) i,
+      ∃ (policy_id : iammodel.PolicyID.t),
+        "Hpolicies" ∷ policies_l ↦${dq_policies} policies ∗
+        "resource" ∷ resource_ptr ↦ resource ∗
+        "policies" ∷ policies_ptr ↦ policies_l ∗
+        "policyID" ∷ policyID_ptr ↦ policy_id ∗
+        "%Hprocessed" ∷ ⌜ ∀ policy_id',
+          policy_id' ∈ list_to_set (C:=gset iammodel.PolicyID.t)
+            (take (Z.to_nat i) keys) →
+          policy_matches_resource policies resource policy_id' = false ⌝)%I
+    (λ bv,
+      ∃ (policy_id : iammodel.PolicyID.t),
+        "Hpolicies" ∷ policies_l ↦${dq_policies} policies ∗
+        "resource" ∷ resource_ptr ↦ resource ∗
+        "policies" ∷ policies_ptr ↦ policies_l ∗
+        "policyID" ∷ policyID_ptr ↦ policy_id ∗
+        "%Hreturn" ∷ ⌜ bv = return_val #true ∧
+          attached_policies_for_resource policies policy_ids resource ≠ ∅ ⌝)%I
+    with "HpolicyIDs").
+  iIntros (keys) "%Hkeys".
+  iSplitL "Hpolicies resource policies policyID".
+  { iExists ""%go. iFrame. iPureIntro.
+    rewrite take_0 list_to_set_nil. intros ? Hin.
+    rewrite elem_of_empty in Hin. done. }
+  iSplitL "".
+  { iModIntro. iIntros (i policy_id []) "%Hiter Hbody".
+    destruct Hiter as [Hi_bounds [Hkey_lookup Hpolicy_id_lookup]].
+    iDestruct "Hbody" as (last_policy_id)
+      "(Hpolicies & resource & policies & policyID & %Hprocessed)".
+    wp_auto.
+    wp_apply (wp_map_lookup2 iammodel.PolicyID iammodel.IdentityPolicy
+      with "[$Hpolicies]").
+    iIntros "Hpolicies".
+    destruct (policies !! policy_id) as [policy|] eqn:Hpolicy_lookup;
+      wp_auto.
+    - destruct (decide
+        (policy.(iammodel.IdentityPolicy.Resource') = resource)) as
+        [Hresource_eq|Hresource_ne].
+      + replace (bool_decide
+          (policy.(iammodel.IdentityPolicy.Resource') = resource)) with true.
+        2:{ symmetry. apply bool_decide_eq_true_2. done. }
+        wp_auto.
+        iRight. iRight. iExists #true. iSplit; [done|].
+        iExists policy_id. iFrame. iPureIntro. split; [done|].
+        intros Hempty.
+        assert (policy_id ∈ attached_policies_for_resource
+          policies policy_ids resource) as Hin.
+        { apply attached_policies_for_resource_elem.
+          split; [exact Hpolicy_id_lookup|].
+          unfold policy_matches_resource. rewrite Hpolicy_lookup.
+          apply bool_decide_eq_true_2. done. }
+        rewrite Hempty elem_of_empty in Hin. done.
+      + replace (bool_decide
+          (policy.(iammodel.IdentityPolicy.Resource') = resource)) with false.
+        2:{ symmetry. apply bool_decide_eq_false_2. done. }
+        wp_auto.
+        iRight. iLeft. iSplit; [done|].
+        iExists policy_id. iFrame. iPureIntro.
+        intros policy_id' Hin.
+        replace (Z.to_nat (i + 1)) with (S (Z.to_nat i)) in Hin by lia.
+        rewrite (take_S_r _ _ _ Hkey_lookup) in Hin.
+        rewrite elem_of_list_to_set elem_of_app /= in Hin.
+        destruct Hin as [Hin|Hin].
+        * apply Hprocessed. rewrite elem_of_list_to_set. exact Hin.
+        * rewrite elem_of_cons elem_of_nil in Hin.
+          destruct Hin as [Heq|[]]. subst policy_id'.
+          unfold policy_matches_resource. rewrite Hpolicy_lookup.
+          apply bool_decide_eq_false_2. done.
+    - iRight. iLeft. iSplit; [done|].
+      iExists policy_id. iFrame. iPureIntro.
+      intros policy_id' Hin.
+      replace (Z.to_nat (i + 1)) with (S (Z.to_nat i)) in Hin by lia.
+      rewrite (take_S_r _ _ _ Hkey_lookup) in Hin.
+      rewrite elem_of_list_to_set elem_of_app /= in Hin.
+      destruct Hin as [Hin|Hin].
+      * apply Hprocessed. rewrite elem_of_list_to_set. exact Hin.
+      * rewrite elem_of_cons elem_of_nil in Hin.
+        destruct Hin as [Heq|[]]. subst policy_id'.
+        unfold policy_matches_resource. rewrite Hpolicy_lookup. done.
+      }
+  iIntros (bv) "HpolicyIDs Hresult".
+  iDestruct "Hresult" as "[Hdone|Hreturn]".
+  - iDestruct "Hdone" as "(-> & Hdone)".
+    iDestruct "Hdone" as (last_policy_id)
+      "(Hpolicies & resource & policies & policyID & %Hprocessed)".
+    assert (attached_policies_for_resource policies policy_ids resource = ∅)
+      as Hempty.
+    { apply attached_policies_for_resource_empty.
+      intros policy_id Hlookup.
+      apply Hprocessed.
+      destruct Hkeys as [Hkeys_dom [Hkeys_len Hkeys_nodup]].
+      rewrite Nat2Z.id.
+      replace (size policy_ids) with (length keys) by done.
+      replace (take (length keys) keys) with keys.
+      2:{ symmetry. apply take_ge. apply Nat.le_refl. }
+      rewrite Hkeys_dom elem_of_dom. eexists. exact Hlookup. }
+    wp_auto.
+    replace (#false) with
+      (#(bool_decide
+        (attached_policies_for_resource policies policy_ids resource ≠ ∅))).
+    2:{ f_equal. apply bool_decide_eq_false_2.
+        rewrite Hempty. intros Hneq. apply Hneq. done. }
+    iApply "HΦ". iFrame.
+  - iDestruct "Hreturn" as (policy_id)
+      "(Hpolicies & resource & policies & policyID & %Hreturn)".
+    destruct Hreturn as [-> Hnonempty].
+    wp_auto.
+    replace (#true) with
+      (#(bool_decide
+        (attached_policies_for_resource policies policy_ids resource ≠ ∅))).
+    2:{ f_equal. apply bool_decide_eq_true_2. done. }
+    iApply "HΦ". iFrame.
+  Unshelve.
+    all: unfold iammodel.PolicyID.t, iammodel.IdentityID.t; apply _.
+Qed.
 
 Lemma wp_identitiesWithPolicyForResource
     identities_l policies_l
@@ -41,8 +276,11 @@ Lemma wp_identitiesWithPolicyForResource
           attached_policies_for_resource policies policy_ids resource ≠ ∅)
           abs_identities) ⌝
   }}}.
-(* FIXME: Proving this needs reusable map.for_range support, including nested
-   map iteration through hasPolicyForResource. *)
+(* FIXME: This callback uses Goose's generated "$value" range temporary.
+   Ordinary function application substitutes the binder "value", leaving
+   "$value" free in the callback body. A sound proof needs either generated
+   callbacks that bind "$value", or a map.for_range semantics/principle that
+   explicitly accounts for this Goose convention. *)
 Proof. Admitted.
 
 Lemma wp_policiesForResource
